extra/LambdaSepSpecExtra.v
@@ -1,0 +1,164 @@
+
+
+(* TODO: not used, to update
+
+(* ---------------------------------------------------------------------- *)
+(** Reformulation of the rule for N-ary functions *)
+
+Definition spec_funs (xs:vars) (t1:trm) (F:val) :=
+  forall (Xs:vals), length xs = length Xs ->
+    triple (substn xs Xs t1) ===> triple (trm_apps F Xs).
+
+Lemma spec_funs_val_funs : forall xs t1,
+  var_distinct xs ->
+  xs <> nil ->
+  spec_funs xs t1 (val_funs xs t1).
+Proof using. introv D N L M. applys* rule_apps_funs. splits~. Qed.
+
+
+(* ---------------------------------------------------------------------- *)
+(** Reformulation of the rule for N-ary recursive functions *)
+
+Definition spec_fixs (f:var) (xs:vars) (t1:trm) (F:val) :=
+  forall (Xs:vals), length xs = length Xs ->
+    triple (subst1 f F (substn xs Xs t1)) ===> triple (trm_apps F Xs).
+
+Lemma spec_fixs_val_fixs : forall f xs t1,
+  var_distinct (f::xs) ->
+  xs <> nil ->
+  spec_fixs f xs t1 (val_fixs f xs t1).
+Proof using. introv D N L M. applys* rule_apps_fixs. splits~. Qed.
+
+
+(* ---------------------------------------------------------------------- *)
+(** Functions of one argument *)
+
+Lemma rule_app_fun : forall x F V t1 H Q,
+  F = (val_fun x t1) ->
+  triple (subst x V t1) H Q ->
+  triple (trm_app F V) H Q.
+Proof using.
+  introv EF M. subst F. intros HF h N.
+  lets~ (h'&v&R&K): (rm M) HF h.
+  exists h' v. splits~. { applys~ red_app_fun. }
+Qed.
+
+Definition spec_fun (x:var) (t1:trm) (F:val) :=
+  forall X, triple (subst x X t1) ===> triple (trm_app F X).
+
+Lemma spec_fun_val_fun : forall x t1,
+  spec_fun x t1 (val_fun x t1).
+Proof using. introv. intros X H Q M. applys* rule_app_fun. Qed.
+
+Lemma rule_fun_spec : forall x t1 H Q,
+  (forall (F:val), spec_fun x t1 F -> H ==> Q F) ->
+  triple (trm_fun x t1) H Q.
+Proof using.
+  introv M. forwards M': (rm M) (val_fun x t1).
+  { applys spec_fun_val_fun. }
+  { applys~ rule_fun. }
+Qed.
+
+
+(* ---------------------------------------------------------------------- *)
+(** Recursive functions of one argument *)
+
+Lemma rule_app_fix : forall f x F V t1 H Q,
+  F = (val_fix f x t1) ->
+  triple (subst f F (subst x V t1)) H Q ->
+  triple (trm_app F V) H Q.
+Proof using.
+  introv EF M. subst F. intros HF h N.
+  lets~ (h'&v&R&K): (rm M) HF h.
+  exists h' v. splits~. { applys~ red_app_fix. }
+Qed.
+
+Definition spec_fix (f:var) (x:var) (t1:trm) (F:val) :=
+  forall X, triple (subst f F (subst x X t1)) ===> triple (trm_app F X).
+
+Lemma spec_fix_val_fix : forall f x t1,
+  spec_fix f x t1 (val_fix f x t1).
+Proof using. introv. intros X H Q M. applys* rule_app_fix. Qed.
+
+Lemma rule_fix_spec : forall f x t1 H Q,
+  (forall (F:val), spec_fix f x t1 F -> H ==> Q F) ->
+  triple (trm_fix f x t1) H Q.
+Proof using.
+  introv M. forwards M': (rm M) (val_fix f x t1).
+  { applys spec_fix_val_fix. }
+  { applys~ rule_fix. }
+Qed.
+
+
+(* ---------------------------------------------------------------------- *)
+(** Functions of two arguments *)
+
+Notation "'val_fun2' x1 x2 t" := (val_fun x1 (trm_fun x2 t))
+  (at level 69, x1 ident, x2 ident, only parsing).
+
+Lemma red_app_fun2 : forall m1 m2 vf v1 v2 x1 x2 t r,
+  vf = val_fun2 x1 x2 t ->
+  red m1 (subst x2 v2 (subst x1 v1 t)) m2 r ->
+  x1 <> x2 ->
+  red m1 (vf v1 v2) m2 r.
+Proof using.
+  hint red_val.
+  introv E M N. subst. applys~ red_app_arg.
+  { applys~ red_app_fun. simpl. case_if. applys red_fun. }
+  { applys~ red_app_fun. }
+Qed.
+
+Definition spec_fun2 (x1 x2:var) (t1:trm) (F:val) :=
+  forall X1 X2, triple (subst x2 X2 (subst x1 X1 t1)) ===> triple (F X1 X2).
+
+Lemma rule_app_fun2 : forall x1 x2 F V1 V2 t1 H Q,
+  F = val_fun2 x1 x2 t1 ->
+  x1 <> x2 ->
+  triple (subst x2 V2 (subst x1 V1 t1)) H Q ->
+  triple (F V1 V2) H Q.
+Proof using.
+  introv E N M. intros H' h Hf. forwards (h'&v&R&K): (rm M) Hf.
+  exists h' v. splits~. { applys* red_app_fun2. }
+Qed.
+
+Lemma spec_fun2_val_fun2 : forall x1 x2 t1,
+  x1 <> x2 ->
+  spec_fun2 x1 x2 t1 (val_fun2 x1 x2 t1).
+Proof using. introv. intros X1 X2 H Q M. applys* rule_app_fun2. Qed.
+
+*)
+
+
+
+(* ---------------------------------------------------------------------- *)
+(** Combination of [rule_let] and [rule_fun] or [rule_fix] *)
+
+
+Lemma rule_let_fun : forall f x t1 t2 H Q,
+  (forall (F:val), spec_fun x t1 F -> triple (subst f F t2) H Q) ->
+  triple (trm_let f (trm_fun x t1) t2) H Q.
+Proof using.
+  introv M. applys rule_let (fun F => \[spec_fun x t1 F] \* H).
+  { applys rule_fun. introv HF. hsimpl~. }
+  { intros F. applys rule_extract_hprop. applys M. }
+Qed.
+
+Lemma rule_let_fix : forall f x t1 t2 H Q,
+  (forall (F:val), spec_fix f x t1 F -> triple (subst f F t2) H Q) ->
+  triple (trm_let f (trm_fix f x t1) t2) H Q.
+Proof using.
+  introv M. applys rule_let (fun F => \[spec_fix f x t1 F] \* H).
+  { applys rule_fix. introv HF. hsimpl~. }
+  { intros F. applys rule_extract_hprop. applys M. }
+Qed.
+
+Lemma rule_let_fun2 : forall f x1 x2 t1 t2 H Q,
+  (forall (F:val), spec_fun2 x1 x2 t1 F -> triple (subst f F t2) H Q) ->
+  x1 <> x2 ->
+  triple (trm_let f (trm_fun x1 (trm_fun x2 t1)) t2) H Q.
+Proof using.
+  introv M N. applys rule_let (fun F => \[spec_fun2 x1 x2 t1 F] \* H).
+  { applys rule_func_val. hsimpl. applys~ spec_fun2_val_fun2. }
+  { intros F. applys rule_extract_hprop. applys M. }
+Qed.
+
