theories/SLRules.v
@@ -45,3 +45,11 @@ Require Import LambdaSemantics LambdaSep.
 (** ** Pure functions *)
 
 (** ** Functions operating on the state *)
+
+
+
+
+
+
+
+
